Sum: some non-dependent data between key and dependent data

src/lowparse/LowParse.SLow.Sum.fst
@@ -191,6 +191,146 @@ let parse32_sum_gen'
 
 #reset-options
 
+module Seq = FStar.Seq
+
+let parse_sum_with_nondep_aux
+  (#kt: parser_kind)
+  (t: sum)
+  (p: parser kt (sum_repr_type t))
+  (#knd: parser_kind)
+  (#nondep_t: Type0)
+  (pnd: parser knd nondep_t)
+  (#k: parser_kind)
+  (pc: ((x: sum_key t) -> Tot (parser k (sum_cases t x))))
+  (input: bytes)
+: GTot (option ((nondep_t * sum_type t) * consumed_length input))
+= match parse (parse_enum_key p (sum_enum t)) input with
+  | Some (tg, consumed_tg) ->
+    let input1 = Seq.slice input consumed_tg (Seq.length input) in
+    begin match parse pnd input1 with
+    | Some (nd, consumed_nd) ->
+      let input2 = Seq.slice input1 consumed_nd (Seq.length input1) in
+      begin match parse (pc tg) input2 with
+      | Some (d, consumed_d) ->
+        Some ((nd, d), consumed_tg + (consumed_nd + consumed_d))
+      | _ -> None
+    end
+    | _ -> None
+    end
+  | _ -> None
+
+#set-options "--z3rlimit 256 --max_fuel 32"
+
+let parse_sum_with_nondep_aux_correct
+  (#kt: parser_kind)
+  (t: sum)
+  (p: parser kt (sum_repr_type t))
+  (#knd: parser_kind)
+  (#nondep_t: Type0)
+  (pnd: parser knd nondep_t)
+  (#k: parser_kind)
+  (pc: ((x: sum_key t) -> Tot (parser k (sum_cases t x))))
+  (input: bytes)
+: Lemma
+  (parse_sum_with_nondep_aux t p pnd pc input == parse (parse_sum_with_nondep t p pnd pc) input)
+=   match parse (parse_enum_key p (sum_enum t)) input with
+    | Some (tg, consumed_tg) ->
+      let input1 = Seq.slice input consumed_tg (Seq.length input) in
+      begin match parse pnd input1 with
+      | Some (nd, consumed_nd) ->
+        let input2 = Seq.slice input1 consumed_nd (Seq.length input1) in
+        begin match parse (pc tg) input2 with
+        | Some (d, consumed_d) ->
+          // FIXME: implicit arguments are not inferred because (synth_tagged_union_data ...) is Tot instead of GTot
+          let (tg' : sum_key (make_sum_with_nondep nondep_t t)) = (tg <: sum_key_type (make_sum_with_nondep nondep_t t)) in
+          let (ndd_ : (nondep_t * sum_type t)) = (nd, (d <: sum_type t)) in
+          let (ndd_ : sum_type (make_sum_with_nondep nondep_t t)) = ndd_ in
+          let u' : sum_key_type (make_sum_with_nondep nondep_t t) = sum_tag_of_data (make_sum_with_nondep nondep_t t) ndd_ in
+          let u : sum_key_type (make_sum_with_nondep nondep_t t) = sum_tag_of_data t (d <: sum_type t) in
+          assert_norm (u' == u);
+          assert (sum_tag_of_data (make_sum_with_nondep nondep_t t) ndd_ == tg');
+          let (ndd : sum_cases (make_sum_with_nondep nondep_t t) tg') = ndd_ in
+          assert_norm (synth_sum_with_nondep_case nondep_t t tg (nd, d) == ndd);
+          let p1 : option (sum_cases (make_sum_with_nondep nondep_t t) tg' * consumed_length input1) = parse (parse_sum_with_nondep_cases t pnd pc tg') input1 in
+          assert (p1 == Some (ndd, consumed_nd + consumed_d));
+//          assert (parse (parse_sum_with_nondep t p pnd pc) input == Some (ndd_, consumed_tg + (consumed_nd + consumed_d)));
+          assert (parse (parse_synth #_ #_ #(sum_type (make_sum_with_nondep nondep_t t)) (parse_sum_with_nondep_cases t pnd pc tg) (synth_tagged_union_data (sum_tag_of_data (make_sum_with_nondep nondep_t t)) tg)) (input1) == Some (ndd_, consumed_nd + consumed_d));
+//          admit
+          ()
+        | _ -> ()
+      end
+      | _ -> ()
+      end
+    | _ -> ()
+
+#reset-options
+
+#set-options "--z3rlimit 32"
+
+inline_for_extraction
+let parse32_sum_with_nondep_aux
+  (#kt: parser_kind)
+  (t: sum)
+  (p: parser kt (sum_repr_type t))
+  (#knd: parser_kind)
+  (#nondep_t: Type0)
+  (#pnd: parser knd nondep_t)
+  (pnd32: parser32 pnd)
+  (#k: parser_kind)
+  (#pc: ((x: sum_key t) -> Tot (parser k (sum_cases t x))))
+  (pc32: ((x: sum_key t) -> Tot (parser32 (pc x))))
+  (p32: parser32 (parse_enum_key p (sum_enum t)))
+  (destr: enum_destr_t (bytes32 -> Tot (option (sum_type t * U32.t))) (feq bytes32 _ (eq2 #(option (sum_type t * U32.t)))) (sum_enum t))
+  (input: bytes32)
+: Tot (option ((nondep_t * sum_type t) * U32.t))
+= match p32 input with
+  | Some (tg, consumed_tg) ->
+    let input1 = b32slice input consumed_tg (B32.len input) in
+    begin match pnd32 input1 with
+    | Some (nd, consumed_nd) ->
+      let input2 = b32slice input1 consumed_nd (B32.len input1) in
+      begin match 
+        destr (fun (x: sum_key t) (input: bytes32) -> match pc32 x input with | Some (d, consumed_d) -> Some ((d <: sum_type t), consumed_d) | _ -> None) tg input2
+      with
+      | Some (d, consumed_d) ->
+        Some ((nd, d), U32.add consumed_tg (U32.add consumed_nd consumed_d))
+      | _ -> None
+    end
+    | _ -> None
+    end
+  | _ -> None
+
+inline_for_extraction
+let parse32_sum_with_nondep_aux_correct
+  (#kt: parser_kind)
+  (t: sum)
+  (p: parser kt (sum_repr_type t))
+  (#knd: parser_kind)
+  (#nondep_t: Type0)
+  (#pnd: parser knd nondep_t)
+  (pnd32: parser32 pnd)
+  (#k: parser_kind)
+  (#pc: ((x: sum_key t) -> Tot (parser k (sum_cases t x))))
+  (pc32: ((x: sum_key t) -> Tot (parser32 (pc x))))
+  (p32: parser32 (parse_enum_key p (sum_enum t)))
+  (destr: enum_destr_t (bytes32 -> Tot (option (sum_type t * U32.t))) (feq bytes32 _ (eq2 #(option (sum_type t * U32.t)))) (sum_enum t))
+  (input: bytes32)
+: Lemma
+  (parser32_correct (parse_sum_with_nondep t p pnd pc) input (parse32_sum_with_nondep_aux t p pnd32 pc32 p32 destr input))
+= let res = parse32_sum_with_nondep_aux t p pnd32 pc32 p32 destr input in
+  let gp = parse_sum_with_nondep_aux t p pnd pc (B32.reveal input) in
+  assert (match res with
+  | None -> gp == None
+  | Some (hres, consumed) ->
+    Some? gp /\ (
+    let (Some (hres', consumed')) = gp in
+    hres == hres' /\
+    U32.v consumed == (consumed' <: nat)
+  ));
+  parse_sum_with_nondep_aux_correct t p pnd pc (B32.reveal input)
+
+#reset-options
+
 inline_for_extraction
 let parse32_sum_gen
   (#kt: parser_kind)
